Add CFG-native VIMP checks and store-only soundness example

src/CFG/CFG_Def.thy
@@ -79,6 +79,7 @@ record cfg =
   intra     :: "(cfg_node \<times> edge_action \<times> cfg_node) set"
   calls     :: "(cfg_node \<times> call_action \<times> cfg_node \<times> cfg_node) set"
   cfg_entry :: cfg_node
+  checks    :: "(cfg_node \<times> bexp) set"
 
 subsection \<open>Intra edge execution\<close>
 
