src/VIMP/VIMP_Proc.thy
@@ -24,6 +24,7 @@ datatype com =
     SKIP
   | Assign (assign_var: vname) (assign_rhs: aexp)
   | Random (random_var: vname)
+  | Check  (check_cond: bexp)
   | Seq    (seq_first: com) (seq_second: com)
   | If     (if_cond: bexp) (if_then: com) (if_else: com)
   | While  (while_cond: bexp) (while_body: com)
@@ -85,6 +86,7 @@ inductive
 where
   Assign:  "pstep gs \<Pi> (Assign x a, s, frs) (SKIP, s(x := aval a s), frs)"
 | Random:  "pstep gs \<Pi> (Random x, s, frs) (SKIP, s(x := v), frs)"
+| Check:   "pstep gs \<Pi> (Check c, s, frs) (SKIP, s, frs)"
 | Seq1:    "pstep gs \<Pi> (Seq SKIP c2, s, frs) (c2, s, frs)"
 | Seq2:    "pstep gs \<Pi> (c1, s, frs) (c1', s', frs')
              \<Longrightarrow> pstep gs \<Pi> (Seq c1 c2, s, frs) (Seq c1' c2, s', frs')"
@@ -130,6 +132,8 @@ inductive_cases AssignSE[elim!]:
   "pstep gs \<Pi> (Assign x a, s, frs) cfg"
 inductive_cases RandomSE[elim!]:
   "pstep gs \<Pi> (Random x, s, frs) cfg"
+inductive_cases CheckSE[elim!]:
+  "pstep gs \<Pi> (Check c, s, frs) cfg"
 inductive_cases SeqSE[elim]:
   "pstep gs \<Pi> (Seq c1 c2, s, frs) cfg"
 inductive_cases IfSE[elim!]:
@@ -191,6 +195,9 @@ lemma pcompletes_assign: "pcompletes gs \<Pi> (Assign x a) s (s(x := aval a s))"
   by (simp add: pcompletes_def)
 
 lemma pcompletes_random: "pcompletes gs \<Pi> (Random x) s (s(x := v))"
+  by (simp add: pcompletes_def)
+
+lemma pcompletes_check: "pcompletes gs \<Pi> (Check c) s s"
   by (simp add: pcompletes_def)
 
 (* -- Sequencing lifts through the small-step --------------------------- *)
@@ -531,6 +538,7 @@ fun com_vnames :: "com => vname set" where
   "com_vnames SKIP = {}"
 | "com_vnames (Assign x a) = insert x (aexp_vnames a)"
 | "com_vnames (Random x) = {x}"
+| "com_vnames (Check c) = bexp_vnames c"
 | "com_vnames (Seq c1 c2) = com_vnames c1 \<union> com_vnames c2"
 | "com_vnames (If b c1 c2) =
     bexp_vnames b \<union> com_vnames c1 \<union> com_vnames c2"
@@ -558,6 +566,9 @@ next
   then show ?case by simp
 next
   case Random
+  then show ?case by simp
+next
+  case Check
   then show ?case by simp
 next
   case Seq
@@ -593,6 +604,7 @@ fun source_com :: "com => bool" where
   "source_com SKIP = True"
 | "source_com (Assign x a) = True"
 | "source_com (Random x) = True"
+| "source_com (Check c) = True"
 | "source_com (Seq c1 c2) = (source_com c1 \<and> source_com c2)"
 | "source_com (If b c1 c2) = (source_com c1 \<and> source_com c2)"
 | "source_com (While b c) = source_com c"
@@ -641,6 +653,7 @@ fun may_fallthrough :: "com => bool" where
   "may_fallthrough SKIP = True"
 | "may_fallthrough (Assign _ _) = True"
 | "may_fallthrough (Random _) = True"
+| "may_fallthrough (Check _) = True"
 | "may_fallthrough (Seq c1 c2) = (may_fallthrough c1 \<and> may_fallthrough c2)"
 | "may_fallthrough (If _ c1 c2) = (may_fallthrough c1 \<or> may_fallthrough c2)"
 | "may_fallthrough (While _ _) = True"
@@ -683,6 +696,7 @@ fun wf_source_com :: "proc_table => com => bool" where
   "wf_source_com \<Pi> SKIP = True"
 | "wf_source_com \<Pi> (Assign x a) = (x \<noteq> ret_var \<and> source_aexp a)"
 | "wf_source_com \<Pi> (Random x) = (x \<noteq> ret_var)"
+| "wf_source_com \<Pi> (Check c) = source_bexp c"
 | "wf_source_com \<Pi> (Seq c1 c2) = (wf_source_com \<Pi> c1 \<and> wf_source_com \<Pi> c2)"
 | "wf_source_com \<Pi> (If b c1 c2) =
      (source_bexp b \<and> wf_source_com \<Pi> c1 \<and> wf_source_com \<Pi> c2)"
