src/CFG/Compiler/Compile_Locality.thy
@@ -468,9 +468,11 @@ proof -
   obtain n2 Emain Kmain
     where mainc: "compile_proc \<Pi> mnm (proc_decl_of [] main) n1 = (n2, Emain, Kmain)"
     by (metis prod_cases3)
+  obtain Cprocs n1' where cprocs: "collect_checks_procs \<Pi> ps 0 = (Cprocs, n1')"
+    by (cases "collect_checks_procs \<Pi> ps 0") auto
   have "intra (compile_prog \<Pi> ps mnm main) = Eprocs \<union> Emain
       \<and> calls (compile_prog \<Pi> ps mnm main) = Kprocs \<union> Kmain"
-    unfolding compile_prog_def by (simp add: procs mainc Let_def)
+    unfolding compile_prog_def by (simp add: procs mainc cprocs Let_def)
   with procs mainc show ?thesis using that by blast
 qed
 
