src/VIMP/VIMP_Notation.thy
@@ -220,6 +220,7 @@ syntax
   "_imp2_assign" :: "id \<Rightarrow> imp2_aexp \<Rightarrow> imp2_stmt"            ("_ := _"                 [900, 61] 61)
   "_imp2_random" :: "id \<Rightarrow> imp2_stmt"                         ("_ := random'(')"        [900] 61)
   "_imp2_return" :: "imp2_aexp \<Rightarrow> imp2_stmt"                  ("return _"               61)
+  "_imp2_check"  :: "imp2_bexp \<Rightarrow> imp2_stmt"                  ("check '( _ ')"          [0] 61)
   "_imp2_if"     :: "imp2_bexp \<Rightarrow> imp2_stmts \<Rightarrow> imp2_stmts \<Rightarrow> imp2_stmt"
                                                                ("if '( _ ') { _ } else { _ }" [0, 61, 61] 61)
   "_imp2_while"  :: "imp2_bexp \<Rightarrow> imp2_stmts \<Rightarrow> imp2_stmt"      ("while '( _ ') { _ }"    [0, 61] 61)
@@ -279,6 +280,7 @@ parse_translation \<open>
     val c_Call   = "VIMP_Proc.com.Call"
     val c_Return = "VIMP_Proc.com.Return"
     val c_Random = "VIMP_Proc.com.Random"
+    val c_Check  = "VIMP_Proc.com.Check"
     val c_proc_decl_of = "VIMP_Proc.proc_decl_of"
 
     val c_None    = "Option.option.None"
@@ -399,6 +401,7 @@ parse_translation \<open>
           K c_Assign $ HOLogic.mk_string x $ aexp_tr a
       | stmt_tr (Const ("_imp2_random", _) $ Free (x, _)) = K c_Random $ HOLogic.mk_string x
       | stmt_tr (Const ("_imp2_return", _) $ e) = K c_Return $ (K c_Some $ aexp_tr e)
+      | stmt_tr (Const ("_imp2_check", _) $ b) = K c_Check $ bexp_tr b
       | stmt_tr (Const ("_imp2_if",     _) $ b $ s1 $ s2) =
           K c_If $ bexp_tr b $ stmts_tr s1 $ stmts_tr s2
       | stmt_tr (Const ("_imp2_while",  _) $ b $ s) = K c_While $ bexp_tr b $ stmts_tr s
